coq/Preservation.v
@@ -13,14 +13,405 @@ From Wasm Require Export ExtendedValidation.
 
 From Wasm.Lib Require Export LibTactics.
 
+
+(* Coercions are too confusing during proofs. *)
+Set Printing Coercions.
+
+
+(**************************************************************)
+(** ** Implicit Types - Copied from ExtendedTyping *)
+
+(* Primary *)
+Implicit Type b : bool.
+Implicit Type n m : nat.
+
+(* Value *)
+Implicit Type val : val.
+Implicit Type vals : list val.
+
+(* Structure *)
+Implicit Type M: module.
+Implicit Type l : labelidx.
+
+Implicit Type instr : instr.
+Implicit Type instrs : list instr.
+Implicit Type f func : func.
+Implicit Type fs funcs : list func.
+Implicit Type tab table: table.
+Implicit Type tabs tables: list table.
+
+(* Type *)
+Implicit Type t : valtype.
+Implicit Type ts : list valtype.
+Implicit Type rt : resulttype.
+Implicit Type bt : blocktype.
+Implicit Type ft functype: functype.
+Implicit Type fts functypes: list functype.
+Implicit Type tt tabletype: tabletype.
+Implicit Type tts tabletypes: list tabletype.
+
+(* Validation *)
+Implicit Type C : context.
+
+(* Execution *)
+Implicit Type cfg : config.
+Implicit Type S : store.
+Implicit Type F : frame.
+Implicit Type T : thread.
+Implicit Type E : eval_context.
+
+Implicit Type ainstr : admin_instr.
+Implicit Type ainstrs : list admin_instr.
+
+Implicit Type fa: funcaddr.
+Implicit Type fas : list funcaddr.
+Implicit Type ta: tableaddr.
+Implicit Type tas : list tableaddr.
+
+Implicit Type fi funcinst: funcinst.
+Implicit Type fis funcinsts: list funcinst.
+Implicit Type ti tableinst: tableinst.
+Implicit Type tis tableinsts: list tableinst.
+
+Implicit Type Mi mi moduleinst: moduleinst.
+
+
+
+(* ================================================================= *)
+(** ** List snoc / app - Aux *)
+
+Fixpoint snoc {X: Type} (l: list X) (x: X) : list X :=
+  match l with
+    | [] => [x]
+    | h :: t => h :: (snoc t x)
+  end.
+
+Lemma length_snoc: forall {X: Type} (l: list X) (x: X),
+  length (snoc l x) = (length l) + 1.
+Proof.
+  intros X l x.
+  induction l as [| x' l' ].
+  reflexivity.
+  simpl.
+  rewrite -> IHl'.
+  reflexivity.
+Qed.
+
+Lemma snoc_eq_app: forall {X: Type} (l: list X) (x: X),
+    snoc l x = l ++ [x].
+Proof.
+  intros X l x.
+  induction l.
+  reflexivity.
+  simpl.
+  rewrite IHl.
+  reflexivity.
+Qed.
+
+Lemma snoc_app: forall {X: Type} (l1 l2: list X) (x: X),
+    snoc (l1 ++ l2) x = l1 ++ snoc l2 x.
+Proof.
+  intros X l1 l2 x.
+  induction l1.
+  reflexivity.
+  simpl.
+  rewrite IHl1.
+  reflexivity.
+Qed.
+
+Lemma snoc_destruct: forall {X: Type} (l1 l2: list X) (x1 x2: X),
+    snoc l1 x1 = snoc l2 x2 ->
+    l1 = l2 /\ x1 = x2.
+Proof.
+  Admitted.
+
+Lemma app_snoc_destruct: forall {X: Type} (l1 l2: list X) (x1 x2: X),
+    l1 ++ [x1] = l2 ++ [x2] ->
+    l1 = l2 /\ x1 = x2.
+Proof.
+  Admitted.
+
+Fixpoint unsnoc {X: Type} (l: list X) : option X :=
+  match l with
+    | [] => None 
+    | [x] => Some x
+    | _ :: xs => (unsnoc xs)
+  end.
+
+Lemma unsnoc_neq: forall {A : Type} (l1 l2 : list A), 
+  unsnoc l1 <> unsnoc l2 ->
+  l1 <> l2.
+Proof. 
+  Admitted.
+
+Lemma unsnoc_snoc_app : forall {X: Type} (l: list X) x,
+    unsnoc (l ++ [x]) = Some x.
+Proof. 
+  Admitted.
+
+Lemma unsnoc_snoc : forall {X: Type} (l: list X) x,
+    unsnoc (snoc l x) = Some x.
+Proof. 
+  Admitted.
+
+
+(* ================================================================= *)
+(** ** Lemma - lifting *)
+
+Lemma lift_up_eq : forall instrs1 instrs2,
+    ↑instrs1 = ↑instrs2 ->
+     instrs1 =  instrs2.
+Proof.
+  Admitted.
+
+Lemma lift_upup_eq : forall vals1 vals2,
+    ⇈vals1 = ⇈vals1 ->
+     vals1 =  vals2.
+Proof.
+  Admitted.
+
+Lemma lift_vals_eq : forall vals1 vals2,
+    lift_vals vals1 = lift_vals vals1 ->
+    vals1 =  vals2.
+Proof.
+  Admitted.
+
+(* using [Lemma map_app] *)
+
+Lemma lift_up_app : forall instrs1 instrs2,
+  ↑(instrs1 ++ instrs2) = ↑instrs1 ++ ↑instrs2.
+Proof.
+  Admitted.
+
+Lemma lift_upup_app : forall vals1 vals2,
+  ⇈(vals1 ++ vals2) = ⇈vals1 ++ ⇈vals2.
+Proof.
+  Admitted.
+
+Lemma lift_vals_app : forall vals1 vals2,
+  lift_vals (vals1 ++ vals2) = lift_vals vals1 ++ lift_vals vals2.
+Proof.
+  Admitted.
+
+
+(* ================================================================= *)
+(** ** Lemma - Aux *)
+
+Lemma plug_E_ϵ : forall E ainstrs, 
+  plug__E E ainstrs = [] ->
+  ainstrs = [].
+Proof.
+  Admitted.
+
+(* if the snoc is [val], then all [val] *)
+Lemma snoc_val_is_normal_form2: forall ainstrs val, 
+  ~ exists ainstrs', ainstrs ++ ⇈[val] ↪s ainstrs'.
+Proof.
+  Admitted.
+      
+Lemma snoc_val_is_normal_form: forall instrs val, 
+  ~ exists ainstrs', ↑(instrs ++ [Const val]) ↪s ainstrs'.
+Proof.
+  Admitted.
+
+
+Lemma S_F_ϵ_is_normal_form : forall S F S' F',
+  ~ exists ainstrs', (S, F, []) ↪ (S', F', ainstrs').
+Proof with auto.
+  introv. intros H.
+  inverts H as. intros ainstrs' HSC.
+
+  (* want both inversion and induction? [remember] *)
+  remember (S, F, []) as S_F_ϵ.     
+
+  induction HSC;
+    inverts HeqS_F_ϵ as.
+
+  - (* SC_simple *)
+    inversion H.
+
+  - (* SC_E *)
+    intros HE.
+    apply plug_E_ϵ in HE; subst.
+    apply IHHSC...
+Qed.
+
+(* We observed this is too strong and we need
+   a specific [C] and [ts1] (via [remember].
+   also to have a specifc [ts1],
+   we need to connect the the resulttype with thread result.
+   and discover this spec bug.
+
+    Lemma decompose : forall C instrs instr__N ts0 ts1 ts ts3,
+        C ⊢* instrs ∈ ts1 --> (ts0 ++ ts) (* ts2 *) ->
+        C ⊢  instr__N ∈ ts --> ts3 ->
+        ∃ instrs' vals, instrs ++ [instr__N] = instrs' ++ vals
+ *)
+     
+Lemma decompose : forall C instrs ts0 ts,
+    C ⊢* instrs ∈ [] --> (ts0 ++ ts) ->
+    exists vals0 vals,
+      map type_of vals0 = ts0 -> (* I probably don't care *)
+      map type_of vals  = ts ->  (* I care *)
+      instrs = map Const (vals0 ++ vals).
+Proof.
+  Admitted.
+
+Lemma all_of_type : forall C instrs ts,
+    C ⊢* instrs ∈ [] --> ts ->
+    exists vals,
+      map type_of vals = ts -> 
+      instrs = map Const vals.
+Proof.
+  Admitted.
+
+
+(* ... *)
+Lemma functype_inv : forall C instr__N ts0 ts1 ts2,
+  C ⊢ instr__N ∈ ts1 --> ts2 ->
+  C ⊢ instr__N ∈ (ts0 ++ ts1) --> (ts0 ++ ts2).
+Proof.
+  Admitted.
+
+
+Lemma drop_singleton_typing: forall C instr__N ts1 ts2,
+    C ⊢* [instr__N] ∈ ts1 --> ts2 ->
+    C ⊢ instr__N ∈ ts1 --> ts2.
+Proof.
+  introv HVIS.
+  inverts HVIS.
+  replace ([instr__N]) with ([] ++ [instr__N]) in H.
+  apply app_snoc_destruct in H.
+  inverts H.
+  inverts H3. apply functype_inv. assumption.
+  apply app_eq_nil in H.
+  inverts H.
+  false H1.
+  reflexivity.
+Qed.
+  
+(* TODO: prov in Numerics.v
+   for binop, testop, relop as well.
+ *)
+Lemma eval_unop_inv : forall op val1 val,
+    eval_unop op val1 = Ok (Some val) ->
+    type_of op = type_of val.
+Proof.
+  Admitted.
+
+
+(* ================================================================= *)
+(** ** Lemmas - Cases *)
+
+
+
+(* ================================================================= *)
+(** ** Main Theorem *)
+
 Theorem preservation : forall S T S' T' rt,
     ⊢c (S, T) ∈ rt ->
     $(S, T) ↪ $(S', T') ->
     ⊢c (S', T') ∈ rt /\ ⊢S S ⪯ S'.
 Proof with eauto.
-  introv Ht.
+  introv HVC.
   gen S' T'.
-  induction Ht; introv Hs; inversion Hs. (* 1356 goals *)
-  Abort.
+  (* valid_config *) inverts HVC as HSok HVT.
+  (* valid_thread *) inverts HVT as HVA HVAIS. 
+     (* valid_frame *) inverts keep HVA as HVMI HVV.  
+     (* valid_admin_instrs *) inverts HVAIS as HVIS.    
 
+  (* Induction on typing derivation of valid_instrs have 2 cases.
+     We need to remember all specifics otherwise they will get lost.
+   *)
+  remember (C0 with_locals = ts with_return = None) as C.
+  remember ([] --> rt) as progtype.
+  induction HVIS as [ | ? ? ? ? ? ? ? HVIS' IHHVIS' HVI__N ]; (* [eqn:H] failed? *)
+    introv HSC;
+    simpl in HSC;
+    remember {| A_locals := vals; A_module := mi |} as F;
+    destruct T' as [F' ainstrs'].
 
+  - (* VIS_empty *)
+    exfalso.
+    apply (S_F_ϵ_is_normal_form S F S' F'). 
+    exists ainstrs'...
+
+  - (* VIS_snoc *)
+    remember (S, F, ↑ (instrs ++ [instr__N])) as SF.
+    remember (S', F', ainstrs') as SF'.
+    induction HSC as [ ? ? ? ? HSS | ];
+      inverts Heqprogtype;
+      inverts HeqSF;
+      inverts HeqSF'.
+      
+    + (* SC_simple *)
+      inverts keep HVI__N. (* invert typing [instrN] *)
+
+      ++ (* VI_const *)
+         exfalso.
+         simpl in HSS.
+         apply (snoc_val_is_normal_form instrs val).
+         exists ainstrs'...
+
+      ++ (* VI_unop *)
+         inverts HSS as. (* invert [step_simple] relation *)
+
+        +++ (* [SS_unop__some] *)
+            introv Heval_unop Heq.
+
+            replace ([Plain (Const val1); Plain (Unop op0)])
+               with (↑([Const val1] ++ [Unop op0])) in Heq.
+            apply lift_up_eq in Heq.
+            apply app_snoc_destruct in Heq.
+            inverts Heq as Heqop; inverts Heqop.
+
+            split.
+            ++++ constructor.
+                 assumption.
+                 subst. (* rewrite <- TEMP. *)
+                 econstructor. apply HVA.
+                 constructor. replace ([Const val]) with ([] ++ [Const val]).
+                 eapply VIS_snoc.
+                 apply drop_singleton_typing in HVIS'.
+                 inverts HVIS'.
+                 skip. (* eapply VIS_empty. *)
+                 apply VI_const.
+                 apply (eval_unop_inv _ val1)...
+                 reflexivity.
+                 trivial.
+            ++++ skip.
+            ++++ simpl. reflexivity.
+
+        +++ (* [SS_unop__none] *)
+            skip.
+           
+        +++ (* contradiction *)
+            intros.
+            replace ([Plain (Const c1); Plain (Const c2); Plain (Binop op0)])
+               with (↑([Const c1; Const c2] ++ [Binop op0])) in H.
+            apply lift_up_eq in H.
+            false H.
+            apply unsnoc_neq in H...
+            replace (unsnoc ([Const c1; Const c2] ++ [Binop op0])) with (Some (Binop op0)). 
+            replace (unsnoc (instrs ++ [Unop op])) with (Some (Unop op)). 
+            unfold not; intros. false H1.
+            skip. (* eapply (unsnoc_snoc_app instrs (Unop op)).  *)
+            skip.  (* eapply unsnoc_snoc_app. *)
+            reflexivity.
+
+        +++ (* contradiction *) skip.
+        +++ (* contradiction *) skip.
+        +++ (* contradiction *) skip.
+
+      (* should be similar with VI_unop,
+         will polish the proof and extract them as lemma. *)
+      ++ (* VI_binop *)
+         admit.
+      ++ (* VI_testop *)
+         admit.
+      ++ (* VI_relop *)
+         admit.
+                                        
+    + (* SC_E *)
+      admit.
+  
