coq/Validation.v
@@ -379,9 +379,9 @@ Inductive valid_instr : context -> instr -> functype -> Prop :=
 (* ----------------------------------------------------------------- *)
 (** *** Numeric Instruction *)
 
-  | VI_const : forall C t v,
-      t = type_of v ->
-      C ⊢ Const v ∈ [] --> [t]
+  | VI_const : forall C t val,
+      t = type_of val ->
+      C ⊢ val ∈ [] --> [t]
 
   | VI_unop : forall C t op,
       t = type_of op ->
@@ -406,26 +406,26 @@ Inductive valid_instr : context -> instr -> functype -> Prop :=
 (* ----------------------------------------------------------------- *)
 (** *** Parametric Instruction *)
 
-  | VI_drop : forall C t,
-      C ⊢ Drop ∈ [t] --> []
+  (* | VI_drop : forall C t, *)
+  (*     C ⊢ Drop ∈ [t] --> [] *)
 
-  | VI_select : forall C t,
-      C ⊢ Select ∈ [t; t; T_i32] --> [t]
+  (* | VI_select : forall C t, *)
+  (*     C ⊢ Select ∈ [t; t; T_i32] --> [t] *)
 
 (* ----------------------------------------------------------------- *)
 (** *** Variable Instruction *)
 
-  | VI_local_get : forall C x t,
-      C.(C_locals).[x] = Some t ->
-      C ⊢ Local_get x ∈ [] --> [t]
+  (* | VI_local_get : forall C x t, *)
+  (*     C.(C_locals).[x] = Some t -> *)
+  (*     C ⊢ Local_get x ∈ [] --> [t] *)
 
-  | VI_local_set : forall C x t,
-      C.(C_locals).[x] = Some t ->
-      C ⊢ Local_set x ∈ [t] --> []
+  (* | VI_local_set : forall C x t, *)
+  (*     C.(C_locals).[x] = Some t -> *)
+  (*     C ⊢ Local_set x ∈ [t] --> [] *)
 
-  | VI_local_tee : forall C x t,
-      C.(C_locals).[x] = Some t ->
-      C ⊢ Local_tee x ∈ [t] --> [t]
+  (* | VI_local_tee : forall C x t, *)
+  (*     C.(C_locals).[x] = Some t -> *)
+  (*     C ⊢ Local_tee x ∈ [t] --> [t] *)
 
 (*
   | VI_global_get : forall C x t,
@@ -443,49 +443,49 @@ Inductive valid_instr : context -> instr -> functype -> Prop :=
 (* ----------------------------------------------------------------- *)
 (** *** Control Instructions *)
 
-  | VI_nop : forall C,
-      C ⊢ Nop ∈ [] --> []
+  (* | VI_nop : forall C, *)
+  (*     C ⊢ Nop ∈ [] --> [] *)
 
-  | VI_unreachable : forall C ts1 ts2,
-      C ⊢ Unreachable ∈ ts1 --> ts2
+  (* | VI_unreachable : forall C ts1 ts2, *)
+  (*     C ⊢ Unreachable ∈ ts1 --> ts2 *)
 
-  | VI_block : forall C bt ts1 ts2 instrs,
-      C ⊢bt bt ∈ ts1 --> ts2 ->
-      C,labels ts2 ⊢* instrs ∈ ts1 --> ts2 ->
-      C ⊢ Block bt instrs ∈ ts1 --> ts2
+  (* | VI_block : forall C bt ts1 ts2 instrs, *)
+  (*     C ⊢bt bt ∈ ts1 --> ts2 -> *)
+  (*     C,labels ts2 ⊢* instrs ∈ ts1 --> ts2 -> *)
+  (*     C ⊢ Block bt instrs ∈ ts1 --> ts2 *)
 
-  | VI_loop : forall C bt ta tr instrs,
-      C ⊢bt bt ∈ ta --> tr ->
-      C,labels ta ⊢* instrs ∈ ta --> tr ->
-      C ⊢ Loop bt instrs ∈ ta --> tr
+  (* | VI_loop : forall C bt ta tr instrs, *)
+  (*     C ⊢bt bt ∈ ta --> tr -> *)
+  (*     C,labels ta ⊢* instrs ∈ ta --> tr -> *)
+  (*     C ⊢ Loop bt instrs ∈ ta --> tr *)
 
-  | VI_if : forall C bt ta tr instrs1 instrs2,
-      C ⊢bt bt ∈ ta --> tr ->
-      C,labels tr ⊢* instrs1 ∈ ta --> tr ->
-      C,labels tr ⊢* instrs2 ∈ ta --> tr ->
-      C ⊢ If bt instrs1 instrs2 ∈ (ta ++ [T_i32]) --> tr
+  (* | VI_if : forall C bt ta tr instrs1 instrs2, *)
+  (*     C ⊢bt bt ∈ ta --> tr -> *)
+  (*     C,labels tr ⊢* instrs1 ∈ ta --> tr -> *)
+  (*     C,labels tr ⊢* instrs2 ∈ ta --> tr -> *)
+  (*     C ⊢ If bt instrs1 instrs2 ∈ (ta ++ [T_i32]) --> tr *)
 
-  | VI_br : forall C l tr ts1 ts2,
-      C.(C_labels).[l] = Some tr ->
-      C ⊢ Br l ∈ (ts1 ++ tr) --> ts2
+  (* | VI_br : forall C l tr ts1 ts2, *)
+  (*     C.(C_labels).[l] = Some tr -> *)
+  (*     C ⊢ Br l ∈ (ts1 ++ tr) --> ts2 *)
 
-  | VI_br_if : forall C l tr, 
-      C.(C_labels).[l] = Some tr ->
-      C ⊢ Br_if l ∈ (tr ++ [T_i32]) --> tr
+  (* | VI_br_if : forall C l tr,  *)
+  (*     C.(C_labels).[l] = Some tr -> *)
+  (*     C ⊢ Br_if l ∈ (tr ++ [T_i32]) --> tr *)
 
-  | VI_br_table : forall C ls l__N tr ts1 ts2, 
-      (* this might be easier via length check *)
-      Forall (fun l => C.(C_labels).[l] <> None) ls ->
-      C.(C_labels).[l__N] = Some tr ->
-      C ⊢ Br_table ls l__N ∈ (ts1 ++ tr ++ [T_i32]) --> ts2
+  (* | VI_br_table : forall C ls l__N tr ts1 ts2,  *)
+  (*     (* this might be easier via length check *) *)
+  (*     Forall (fun l => C.(C_labels).[l] <> None) ls -> *)
+  (*     C.(C_labels).[l__N] = Some tr -> *)
+  (*     C ⊢ Br_table ls l__N ∈ (ts1 ++ tr ++ [T_i32]) --> ts2 *)
 
-  | VI_return : forall C tr ts1 ts2,
-      C.(C_return) = Some tr ->
-      C ⊢ Return ∈ (ts1 ++ tr) --> ts2
+  (* | VI_return : forall C tr ts1 ts2, *)
+  (*     C.(C_return) = Some tr -> *)
+  (*     C ⊢ Return ∈ (ts1 ++ tr) --> ts2 *)
 
-  | VI_call : forall C x ts1 ts2,
-      C.(C_funcs).[x] = Some (ts1 --> ts2) ->
-      C ⊢ Call x ∈ ts1 --> ts2
+  (* | VI_call : forall C x ts1 ts2, *)
+  (*     C.(C_funcs).[x] = Some (ts1 --> ts2) -> *)
+  (*     C ⊢ Call x ∈ ts1 --> ts2 *)
 
 (*
   | VI_call_indirect : forall C x ts1 ts2,
@@ -504,8 +504,8 @@ with valid_instrs : context -> list instr -> functype -> Prop :=
       C ⊢* [] ∈ ts --> ts
 
   | VIS_snoc : forall C instrs instr__N ts0 ts1 ts ts3,
-      C ⊢ instr__N ∈ ts --> ts3 ->
-      C ⊢* instrs ∈ ts1 --> (ts0 ++ ts) ->
+      C ⊢* instrs ∈ ts1 --> (ts0 ++ ts) (* ts2 *) ->
+      C ⊢  instr__N ∈ ts --> ts3 ->
       C ⊢* instrs ++ [instr__N] ∈ ts1 --> (ts0 ++ ts3)
 
 where "C '⊢' instr '∈' ft" := (valid_instr C instr ft)
